successfully turned tttree into a map

btree.dfy
@@ -111,8 +111,8 @@ function method seq_union<T>(s: seq<set<T> >) : set<T>
 
 ////////////////////////////////////////////
 
-datatype Node =
-	Leaf(keys: seq<string>, values: seq<int>) |
+datatype Node<Value> =
+	Leaf(keys: seq<string>, values: seq<Value>) |
 	Index(pivots: seq<string>, children: seq<Node>)
 
 predicate subtree_is_well_formed(node: Node) {
@@ -197,19 +197,23 @@ lemma children_have_one_less_height(node: Node)
 	}
 }
 
-predicate is_child_list(nodes: seq<Node>)
+predicate is_child_list(pivots: seq<string>, nodes: seq<Node>)
 {
 	|nodes| > 0 &&
+		|pivots| == |nodes| - 1 &&
 		(forall node :: node in nodes ==> subtree_is_well_formed(node)) &&
 		(forall node :: node in nodes ==> subtree_is_balanced(node)) &&
-		(forall node :: node in nodes ==> height(node) == height(nodes[0]))
+		(forall node :: node in nodes ==> height(node) == height(nodes[0])) &&
+		(
+		forall i :: 0 <= i < |nodes| - 1 ==> forall k :: k in set_of_keys(nodes[i]) ==> lexical_cmp(k, pivots[i]) < 0) &&
+		(forall i :: 1 <= i < |nodes| ==> forall k :: k in set_of_keys(nodes[i]) ==> lexical_cmp(pivots[i-1], k) <= 0)
 }
 
-function set_of_keys_of_children(nodes: seq<Node>) : set<string>
-	requires is_child_list(nodes);
+function set_of_keys_of_children(pivots: seq<string>, nodes: seq<Node>) : set<string>
+	requires is_child_list(pivots, nodes);
 {
 	if |nodes| == 1 then set_of_keys(nodes[0])
-	else set_of_keys(nodes[0]) + set_of_keys_of_children(nodes[1..])
+	else set_of_keys(nodes[0]) + set_of_keys_of_children(pivots[1..], nodes[1..])
 }
 
 function set_of_keys(node: Node) : set<string>
@@ -221,7 +225,7 @@ function set_of_keys(node: Node) : set<string>
 			set k | k in multiset(keys)
 		case Index(pivots, children) =>
 			children_have_one_less_height(node);
-			set_of_keys_of_children(children)
+			set_of_keys_of_children(pivots, children)
 	}
 }
 
@@ -267,40 +271,73 @@ predicate subtree_is_b_tree(node: Node) {
 		subtree_is_sorted(node)
 }
 
-function map_of_kvpairs(acc: map<string, int>, keys: seq<string>, values: seq<int>) : map<string, int>
-	requires |keys| == |values|;
+function merge_disjoint_maps<U,T>(mapa: map<U,T>, mapb: map<U,T>) : map<U,T>
+	requires mapa.Keys !! mapb.Keys;
+	ensures merge_disjoint_maps(mapa, mapb).Keys == mapa.Keys + mapb.Keys;
+	ensures forall k :: k in merge_disjoint_maps(mapa, mapb).Keys && k in mapa.Keys ==>
+		merge_disjoint_maps(mapa, mapb)[k] == mapa[k];
+	ensures forall k :: k in merge_disjoint_maps(mapa, mapb).Keys && k in mapb.Keys ==>
+		merge_disjoint_maps(mapa, mapb)[k] == mapb[k];
 {
-	if |keys| == 0 then acc
-	else map_of_kvpairs(acc, keys[1..], values[1..])[keys[0] := values[0]]
+	map x : U | (x in mapa.Keys + mapb.Keys) :: if x in mapa then mapa[x] else mapb[x]
 }
 
-function map_of_children(acc: map<string, int>, nodes: seq<Node>) : map<string, int>
-	requires is_child_list(nodes);
-	requires forall child :: child in nodes ==> subtree_is_sorted(child);
+function map_of_kvpairs<Value>(keys: seq<string>, values: seq<Value>) : map<string, Value>
+	requires |keys| == |values|;
+	requires seq_is_strictly_increasing(keys);
+	ensures forall k :: k in map_of_kvpairs(keys, values) <==> k in keys;
+	ensures forall k :: k in map_of_kvpairs(keys, values) ==>
+		(exists i :: 0 <= i < |keys| && k == keys[i] && map_of_kvpairs(keys, values)[k] == values[i]);
+{
+	if |keys| == 0 then map[]
+	else map_of_kvpairs(keys[1..], values[1..])[keys[0] := values[0]]
+}
+
+function map_of_children<Value>(pivots: seq<string>, nodes: seq<Node<Value> >) : map<string, Value>
+	requires is_child_list(pivots, nodes);
+	requires forall node :: node in nodes ==> subtree_is_b_tree(node);
+	ensures map_of_children(pivots, nodes).Keys == set_of_keys_of_children(pivots, nodes);
 	decreases height(nodes[0]), |nodes|, 1;
 {
-	if |nodes| == 1 then map_of_subtree(acc, nodes[0])
-	else map_of_children(map_of_subtree(acc, nodes[0]), nodes[1..])
+	if |nodes| == 1 then map_of_subtree(nodes[0])
+	else
+		var map1 := map_of_subtree(nodes[0]);
+		assert forall k :: k in set_of_keys(nodes[0]) ==> lexical_cmp(k, pivots[0]) < 0;
+		assert map1.Keys == set_of_keys(nodes[0]);
+		assert forall k :: k in map1.Keys ==> lexical_cmp(k, pivots[0]) < 0;
+		var map2 := map_of_children(pivots[1..], nodes[1..]);
+		assert map2.Keys == set_of_keys_of_children(pivots[1..], nodes[1..]);
+		assert forall k :: k in map2.Keys ==> lexical_cmp(pivots[0], k) <= 0;
+		merge_disjoint_maps(map1, map2)
 }
 
-function map_of_subtree(acc: map<string, int>, node: Node) : map<string, int>
+function map_of_subtree<Value>(node: Node<Value>) : map<string, Value>
 	requires subtree_is_b_tree(node);
+	ensures map_of_subtree(node).Keys == set_of_keys(node);
 	decreases height(node), 0;
 {
 	match node {
 		case Leaf(keys, values) =>
-			map_of_kvpairs(acc, keys, values)
+			map_of_kvpairs(keys, values)
 		case Index(pivots, children) =>
 			children_have_one_less_height(node);
-			map_of_children(acc, children)
+			map_of_children(pivots, children)
 	}
 }
 
-function subtree_map_contents(node: Node) : map<string, int>
-	requires subtree_is_b_tree(node);
-{
-	map_of_subtree(map[], node)
-}
+// lemma subtree_map_delegation(node: Node, key: string, index: int)
+// 	requires subtree_is_b_tree(node);
+// 	requires node.Index?;
+// 	requires 0 <= index <= |node.pivots|;
+// 	requires forall i :: 0 <= i < index ==> lexical_cmp(node.pivots[i], key) <= 0;
+// 	requires forall i :: index <= i < |node.pivots| ==> lexical_cmp(key, node.pivots[i]) < 0;
+// 	ensures true;
+// 	// ensures key in subtree_map_contents(node) <==> key in subtree_map_contents(node.children[index]);
+// 	// ensures key in subtree_map_contents(node) ==>
+// 	// 	subtree_map_contents(node)[key] == subtree_map_contents(node.children[index])[key];
+// {
+// 	assert forall k :: k in subtree_map_contents(node) ==> k in set_of_keys(node);
+// }
 
 datatype Config = Config(
 	min_leaf_size: int, max_leaf_size: int,
@@ -323,19 +360,19 @@ predicate subtree_satisfies_config(node: Node, cfg: Config)
 	}
 }
 
-datatype QueryResult = KeyDoesNotExist | Value(v: int)
+datatype QueryResult<Value> = KeyDoesNotExist | ValueForKey(v: Value)
 
 	// TODO: binary search
-function method search_seq(keys: seq<string>, values: seq<int>, key: string) : QueryResult
+function method search_seq<Value>(keys: seq<string>, values: seq<Value>, key: string) : QueryResult<Value>
 	requires seq_is_strictly_increasing(keys);
 	requires |keys| == |values|;
-	ensures key !in map_of_kvpairs(map[], keys, values) ==>
+	ensures key !in map_of_kvpairs(keys, values) ==>
 		search_seq(keys, values, key) == KeyDoesNotExist;
-	ensures key in map_of_kvpairs(map[], keys, values) ==>
-		search_seq(keys, values, key) == Value(map_of_kvpairs(map[], keys, values)[key]);
+	ensures key in map_of_kvpairs(keys, values) ==>
+		search_seq(keys, values, key) == ValueForKey(map_of_kvpairs(keys, values)[key]);
 {
 	if |keys| == 0 then KeyDoesNotExist
-	else if keys[0] == key then Value(values[0])
+	else if keys[0] == key then ValueForKey(values[0])
 	else search_seq(keys[1..], values[1..], key)
 }
 
@@ -359,16 +396,16 @@ method search_seq_for_least_greater(keys: seq<string>, key: string) returns (r: 
 	}
 }
 
-method query(node: Node, key: string) returns (qr: QueryResult)
-	requires subtree_is_b_tree(node);
-	ensures key !in subtree_map_contents(node) <==> qr == KeyDoesNotExist;
-	ensures key in subtree_map_contents(node) <==> qr == Value(subtree_map_contents(node)[key]);
-{
-	match node {
-		case Leaf(keys, values) =>
-			qr := search_seq(keys, values, key);
-		case Index(pivots, children) =>
-			var i := search_seq_for_least_greater(pivots, key);
-			qr := query(children[i], key);
-	}
-}
+// method query(node: Node, key: string) returns (qr: QueryResult)
+// 	requires subtree_is_b_tree(node);
+// 	ensures key !in subtree_map_contents(node) <==> qr == KeyDoesNotExist;
+// 	ensures key in subtree_map_contents(node) <==> qr == Value(subtree_map_contents(node)[key]);
+// {
+// 	match node {
+// 		case Leaf(keys, values) =>
+// 			qr := search_seq(keys, values, key);
+// 		case Index(pivots, children) =>
+// 			var i := search_seq_for_least_greater(pivots, key);
+// 			qr := query(children[i], key);
+// 	}
+// }
